indexed_vlsm.v
@@ -185,7 +185,7 @@ Definition indexed_plsm
 Definition indexed_transition
   {index : Set} {message : Type} `{Heqd : EqDec index}
   {IS : index -> LSM_sig message}
-  (IM : forall i : index, @VLSM message (IS i))
+  (IL : forall i : index, @LSM message (IS i))
   (Hinh : inhabited index)
   (l : @label _ (indexed_sig IS Hinh))
   (som : @state _ (indexed_sig IS Hinh) * option (@proto_message _ (indexed_sig IS Hinh)))
@@ -201,10 +201,22 @@ destruct om as [[m _]|].
     exact (state_update s i si', option_map (lift_proto_messageI IS i) om').
 Defined.
 
+
+Definition indexed_lsm
+  {index : Set} {message : Type} `{Heqd : EqDec index}
+  {IS : index -> LSM_sig message}
+  (IL : forall i : index, @LSM message (IS i))
+  (Hi : inhabited index)
+  : @LSM message (indexed_sig IS Hi)
+  :=
+  {|  transition := indexed_transition IL Hi
+  |}.
+
 Definition indexed_valid
   {index : Set} {message : Type} `{Heqd : EqDec index}
   {IS : index -> LSM_sig message}
-  (IM : forall i : index, @VLSM message (IS i))
+  {IL : forall i : index, @LSM message (IS i)}
+  (IM : forall i : index, @VLSM message _ (IL i))
   (Hinh : inhabited index)
   (l : @label _ (indexed_sig IS Hinh))
   (som : @state _ (indexed_sig IS Hinh) * option (@proto_message _ (indexed_sig IS Hinh)))
@@ -223,23 +235,24 @@ Defined.
 Definition indexed_vlsm
   {index : Set} {message : Type} `{Heqd : EqDec index}
   {IS : index -> LSM_sig message}
-  (IM : forall i : index, @VLSM message (IS i))
+  {IL : forall i : index, @LSM message (IS i)}
+  (IM : forall i : index, @VLSM message _ (IL i))
   (Hi : inhabited index)
-  : @VLSM message (indexed_sig IS Hi)
+  : @VLSM message _ (indexed_lsm IL Hi)
   :=
-  {|  transition := indexed_transition IM Hi
-  ;   valid := indexed_valid IM Hi
+  {|  valid := indexed_valid IM Hi
   |}.
 
 Definition indexed_valid_decidable
   {index : Set} {message : Type} `{Heqd : EqDec index}
   {IS : index -> LSM_sig message}
-  {IM : forall i : index, @VLSM message (IS i)}
-  (IDM : forall i : index, @VLSM_vdecidable _ _ (IM i))
+  {IL : forall i : index, @LSM message (IS i)}
+  {IM : forall i : index, @VLSM message _ (IL i)}
+  (IDM : forall i : index, @VLSM_vdecidable _ _ _ (IM i))
   (Hinh : inhabited index)
   (l : @label _ (indexed_sig IS Hinh))
   (som : @state _ (indexed_sig IS Hinh) * option (@proto_message _ (indexed_sig IS Hinh)))
-  : {@valid _ _ (indexed_vlsm IM Hinh) l som} + {~@valid _ _ (indexed_vlsm IM Hinh) l som}.
+  : {@valid _ _ _ (indexed_vlsm IM Hinh) l som} + {~@valid _ _ _ (indexed_vlsm IM Hinh) l som}.
 destruct som as [s om].
 destruct l as [i li]; simpl.
 destruct om as [[m _]|]; simpl.
@@ -252,10 +265,11 @@ Defined.
 Definition indexed_vlsm_vdecidable
   {index : Set} {message : Type} `{Heqd : EqDec index}
   {IS : index -> LSM_sig message}
-  {IM : forall i : index, @VLSM message (IS i)}
-  (IDM : forall i : index, @VLSM_vdecidable _ _ (IM i))
+  {IL : forall i : index, @LSM message (IS i)}
+  {IM : forall i : index, @VLSM message _ (IL i)}
+  (IDM : forall i : index, @VLSM_vdecidable _ _ _ (IM i))
   (Hi : inhabited index)
-  : @VLSM_vdecidable _ _ (indexed_vlsm IM Hi)
+  : @VLSM_vdecidable _ _ _ (indexed_vlsm IM Hi)
   :=
   {|  valid_decidable := indexed_valid_decidable IDM Hi
   |}.
@@ -288,7 +302,8 @@ Definition indexed_plsm_constrained
 Definition indexed_valid_constrained
   {index : Set} {message : Type} `{Heqd : EqDec index}
   {IS : index -> LSM_sig message}
-  (IM : forall i : index, @VLSM message (IS i))
+  {IL : forall i : index, @LSM message (IS i)}
+  (IM : forall i : index, @VLSM message _ (IL i))
   (Hinh : inhabited index)
   (constraint : indexed_label IS -> indexed_state IS * option (indexed_proto_message IS) -> Prop)
   (l : @label _ (indexed_sig IS Hinh))
@@ -302,26 +317,27 @@ Definition indexed_valid_constrained
 Definition indexed_vlsm_constrained
   {index : Set} {message : Type} `{Heqd : EqDec index}
   {IS : index -> LSM_sig message}
-  (IM : forall i : index, @VLSM message (IS i))
+  {IL : forall i : index, @LSM message (IS i)}
+  (IM : forall i : index, @VLSM message _ (IL i))
   (Hi : inhabited index)
   (constraint : indexed_label IS -> indexed_state IS * option (indexed_proto_message IS) -> Prop)
-  : @VLSM message (indexed_sig IS Hi)
+  : @VLSM message _ (indexed_lsm IL Hi)
   :=
-  {|  transition := indexed_transition IM Hi
-  ;   valid := indexed_valid_constrained IM Hi constraint
+  {|  valid := indexed_valid_constrained IM Hi constraint
   |}.
 
 Definition indexed_valid_constrained_decidable
   {index : Set} {message : Type} `{Heqd : EqDec index}
   {IS : index -> LSM_sig message}
-  {IM : forall i : index, @VLSM message (IS i)}
-  (IDM : forall i : index, @VLSM_vdecidable _ _ (IM i))
+  {IL : forall i : index, @LSM message (IS i)}
+  {IM : forall i : index, @VLSM message _ (IL i)}
+  (IDM : forall i : index, @VLSM_vdecidable _ _ _ (IM i))
   (Hinh : inhabited index)
   {constraint : indexed_label IS -> indexed_state IS * option (indexed_proto_message IS) -> Prop}
   (constraint_decidable : forall (l : indexed_label IS) (som : indexed_state IS * option (indexed_proto_message IS)), {constraint l som} + {~constraint l som})
   (l : @label _ (indexed_sig IS Hinh))
   (som : @state _ (indexed_sig IS Hinh) * option (@proto_message _ (indexed_sig IS Hinh)))
-  : {@valid _ _ (indexed_vlsm_constrained IM Hinh constraint) l som} + {~@valid _ _ (indexed_vlsm_constrained IM Hinh constraint) l som}.
+  : {@valid _ _ _ (indexed_vlsm_constrained IM Hinh constraint) l som} + {~@valid _ _ _ (indexed_vlsm_constrained IM Hinh constraint) l som}.
 intros.
 unfold indexed_valid_constrained.
 destruct (constraint_decidable l som) as [Hc | Hnc].
@@ -334,12 +350,13 @@ Defined.
 Definition indexed_vlsm_constrained_vdecidable
   {index : Set} {message : Type} `{Heqd : EqDec index}
   {IS : index -> LSM_sig message}
-  {IM : forall i : index, @VLSM message (IS i)}
-  (IDM : forall i : index, @VLSM_vdecidable _ _ (IM i))
+  {IL : forall i : index, @LSM message (IS i)}
+  {IM : forall i : index, @VLSM message _ (IL i)}
+  (IDM : forall i : index, @VLSM_vdecidable _ _ _ (IM i))
   (Hinh : inhabited index)
   {constraint : indexed_label IS -> indexed_state IS * option (indexed_proto_message IS) -> Prop}
   (constraint_decidable : forall (l : indexed_label IS) (som : indexed_state IS * option (indexed_proto_message IS)), {constraint l som} + {~constraint l som})
-  : @VLSM_vdecidable _ _ (indexed_vlsm_constrained IM Hinh constraint)
+  : @VLSM_vdecidable _ _ _ (indexed_vlsm_constrained IM Hinh constraint)
   :=
   {|  valid_decidable := indexed_valid_constrained_decidable IDM Hinh constraint_decidable
   |}.
@@ -348,8 +365,9 @@ Definition indexed_vlsm_constrained_vdecidable
 Lemma indexed_partial_composition_commute
   {index : Set} {message : Type} `{Heqd : EqDec index}
   {IS : index -> LSM_sig message}
-  {IM : forall i : index, @VLSM message (IS i)}
-  (IDM : forall i : index, @VLSM_vdecidable _ _ (IM i))
+  {IL : forall i : index, @LSM message (IS i)}
+  {IM : forall i : index, @VLSM message _ (IL i)}
+  (IDM : forall i : index, @VLSM_vdecidable _ _ _ (IM i))
   (Hinh : inhabited index)
   : let PM12 := DVLSM_PLSM_instance (indexed_vlsm_vdecidable IDM Hinh) in
     let PM12' := indexed_plsm (fun (i : index) => DVLSM_PLSM_instance (IDM i)) Hinh in
@@ -377,8 +395,9 @@ Qed.
 Lemma indexed_constrained_partial_composition_commute
   {index : Set} {message : Type} `{Heqd : EqDec index}
   {IS : index -> LSM_sig message}
-  {IM : forall i : index, @VLSM message (IS i)}
-  (IDM : forall i : index, @VLSM_vdecidable _ _ (IM i))
+  {IL : forall i : index, @LSM message (IS i)}
+  {IM : forall i : index, @VLSM message _ (IL i)}
+  (IDM : forall i : index, @VLSM_vdecidable _ _ _ (IM i))
   (Hinh : inhabited index)
   {constraint : @label _ (indexed_sig IS Hinh) -> @state _ (indexed_sig IS Hinh) * option (@proto_message _ (indexed_sig IS Hinh)) -> Prop}
   (constraint_decidable : forall (l : @label _ (indexed_sig IS Hinh)) (som : @state _ (indexed_sig IS Hinh) * option (@proto_message _ (indexed_sig IS Hinh))), {constraint l som} + {~constraint l som})
