indexed_vlsm_projections.v
@@ -4,16 +4,19 @@ Require Import vlsm vlsm_preamble composed_vlsm composed_vlsm_projections indexe
 Definition indexed_vlsm_projection
   {message : Type}
   {oindex : Set} {message : Type} `{Heqd : EqDec oindex}
-  (IS : oindex -> LSM_sig message)
-  (IM : forall i : oindex, @VLSM message (IS i))
+  {IS : oindex -> LSM_sig message}
+  {IL : forall i : oindex, @LSM message (IS i)}
+  (IM : forall i : oindex, @VLSM message _ (IL i))
   (i : oindex)
   : VLSM (message : Type)
   :=
   @vlsm_projection message
     (indexed_sig IS (inhabits i))
     (indexed_sig_composed_instance IS (inhabits i))
+    (indexed_lsm IL (inhabits i))
+    (indexed_lsm_composed_instance IL (inhabits i))
     (indexed_vlsm IM (inhabits i))
-    (@indexed_vlsm_composed_instance oindex message Heqd IS IM (inhabits i))
+    (@indexed_vlsm_composed_instance oindex message Heqd IS IL IM (inhabits i))
     i
   .
 
